\begin{enumerate}
    \item Let $M = x, N = \mathsf{h}(y)$. \\
        $(x = \mathsf{h}(\mathsf{senc}(a, k)) \neq_{E_{enc}} \mathsf{h}(y))_{\varphi_1}$
        and
        $(x =_{E_{enc}} \mathsf{h}(y))_{\varphi_2}
        \implies \varphi_1 \centernot\sim \varphi_2$
    \item Let $M = x, N = \mathsf{aenc}(\langle z, c \rangle, y)$. \\
        $(x =_{E_{enc}} \mathsf{aenc}(\langle z, c \rangle, y))_{\varphi_1}$
        and
        $(x = \mathsf{aenc}(\langle \mathsf{senc}(b, k), c \rangle, y) \neq_{E_{enc}} \mathsf{aenc}(\langle z, c \rangle, y))\varphi_1)_{\varphi_2} \\
        \implies \varphi_1 \centernot\sim \varphi_2$
\end{enumerate}
